theories/ordinals/Ackermann/PA.v
@@ -117,7 +117,6 @@ Proof.
                    try (right; unfold not in |- *; intros; 
                         decompose record H; discriminate H1).
                (*   do 4 fold impH  in |- *. *)
-                 do 4 fold forallH in |- *.
                  induction (formula_dec LNT LNT_dec
                               (substituteFormula LNT f1 n0 Zero) f).
                  rewrite <- a.
