theories/ordinals/Ackermann/fol.v
@@ -715,5 +715,6 @@ Arguments Terms_Term_rec_full L P P0 : rename.
 
 Arguments impH {L} _ _.
 Arguments notH {L} _.
+Arguments forallH {L} _ _.
 
 
