theories/ordinals/Ackermann/folLogic2.v
@@ -21,7 +21,6 @@ Let var := var L.
 Let apply := apply L.
 Let equal := equal L.
 Let atomic := atomic L.
-Let forallH := forallH L.
 Let orH := orH L.
 Let andH := andH L.
 Let existH := existH L.
@@ -147,7 +146,7 @@ Proof.
              newVar
                (v1
                   :: v2
-                  :: freeVarFormula L (fol.forallH L v a) ++
+                  :: freeVarFormula L (forallH v a) ++
                   freeVarTerm L s1 ++ freeVarTerm L s2)) in *.
       assert (H2: v' <> v1).
       { intro H2;
@@ -155,7 +154,7 @@ Proof.
           (newVar1
              (v1
                 :: v2
-                :: freeVarFormula L (fol.forallH L v a) ++
+                :: freeVarFormula L (forallH v a) ++
                 freeVarTerm L s1 ++ freeVarTerm L s2)).
         fold v' ; simpl; auto.
       } 
@@ -165,17 +164,17 @@ Proof.
           (newVar1
              (v1
                 :: v2
-                :: freeVarFormula L (fol.forallH L v a) ++
+                :: freeVarFormula L (forallH v a) ++
                 freeVarTerm L s1 ++ freeVarTerm L s2)).
         fold v'; simpl; auto.
       } 
-      assert (H4: ~ In v' (freeVarFormula L (fol.forallH L v a))).
+      assert (H4: ~ In v' (freeVarFormula L (forallH v a))).
       { intro H4; 
         elim
           (newVar1
              (v1
                 :: v2
-                :: freeVarFormula L (fol.forallH L v a) ++
+                :: freeVarFormula L (forallH v a) ++
                 freeVarTerm L s1 ++ freeVarTerm L s2)).
         fold v' ;simpl; auto with datatypes.
       } 
@@ -185,7 +184,7 @@ Proof.
           (newVar1
              (v1
                 :: v2
-                :: freeVarFormula L (fol.forallH L v a) ++
+                :: freeVarFormula L (forallH v a) ++
                 freeVarTerm L s1 ++ freeVarTerm L s2)).
         fold v' ;  simpl; repeat right; auto with datatypes.
       } 
@@ -195,7 +194,7 @@ Proof.
             (newVar1
                (v1
                   :: v2
-                  :: freeVarFormula L (fol.forallH L v a) ++
+                  :: freeVarFormula L (forallH v a) ++
                   freeVarTerm L s1 ++ freeVarTerm L s2)).
        fold v' ; simpl;  repeat right; auto with datatypes.
      }
@@ -203,17 +202,17 @@ Proof.
        (iffH
           (substituteFormula L
              (substituteFormula L
-                (fol.forallH L v' (substituteFormula L a v (var v'))) v1 s1) v2
+                (forallH v' (substituteFormula L a v (var v'))) v1 s1) v2
              s2)
           (substituteFormula L
              (substituteFormula L
-                (fol.forallH L v' (substituteFormula L a v (var v'))) v2 s2) v1
+                (forallH v' (substituteFormula L a v (var v'))) v2 s2) v1
              (substituteTerm L s1 v2 s2))).
      apply (iffE2 L).
       * assert
           (H7: folProof.SysPrf L (Empty_set Formula)
-                 (iffH (fol.forallH L v a)
-                    (fol.forallH L v' (substituteFormula L a v (var v')))))
+                 (iffH (forallH v a)
+                    (forallH v' (substituteFormula L a v (var v')))))
           by (apply rebindForall; auto).
        repeat first
        [ apply (reduceIff L)
