theories/ordinals/Ackermann/folProof.v
@@ -18,7 +18,6 @@ Let apply := apply L.
 Let equal := equal L.
 Let atomic := atomic L.
 Let iffH := iffH L.
-Let forallH := forallH L.
 
 Fixpoint nVars (n: nat) : Terms n * Terms n:=
   match n with 
