theories/ordinals/Ackermann/folProp.v
@@ -19,8 +19,6 @@ Let var := var L.
 Let apply := apply L.
 Let equal := equal L.
 Let atomic := atomic L.
-
-Let forallH := forallH L.
 Let lt_depth := lt_depth L.
 
 Section Free_Variables.
