theories/ordinals/MoreAck/fol_Examples.v
@@ -173,7 +173,7 @@ Print t1_0.
 (** forall v0, v0 = 0 \/ exists v1,  v0 = S v1 *)
 (* begin snippet f1Example *)
 Let f1 : Formula LNN :=
-      forallH LNN 0 
+      forallH 0 
         (orH _ (equal _ (var _ 0) (apply LNN Zero (Tnil _)))
            (existH _ 1 (equal _ (var _ 0)
                           (apply LNN Succ 
